code/Yazi.Adler32.fsti
@@ -1,7 +1,9 @@
 module Yazi.Adler32
 module B = LowStar.Buffer
+module Cast = FStar.Int.Cast
 module Spec = Spec.Adler32
 module U32 = FStar.UInt32
+module U64 = FStar.UInt64
 module U8 = FStar.UInt8
 module Seq = FStar.Seq
 module HS = FStar.HyperStack
@@ -27,3 +29,23 @@ val adler32:
   (ensures fun h0 res h1 ->
     B.(modifies loc_none h0 h1) /\
     Spec.adler32_matched #(m + U32.v len) (Seq.append data (B.as_seq h1 buf)) res)
+
+val adler32_combine64:
+    #m1: Ghost.erased nat
+  -> #m2: Ghost.erased nat
+  -> s1: Ghost.erased (Spec.input m1)
+  -> s2: Ghost.erased (Spec.input m2)
+  -> adler1: U32.t{Spec.adler32_matched s1 adler1}
+  -> adler2: U32.t{Spec.adler32_matched s2 adler2}
+  -> len2: U64.t{U64.v len2 == Ghost.reveal m2}
+  -> Tot (res: U32.t{Spec.adler32_matched #(m1 + m2) (Seq.append s1 s2) res})
+
+inline_for_extraction
+let adler32_combine
+  (#m1 #m2: Ghost.erased nat)
+  (s1: Ghost.erased (Spec.input m1))
+  (s2: Ghost.erased (Spec.input m2))
+  (adler1: U32.t{Spec.adler32_matched s1 adler1})
+  (adler2: U32.t{Spec.adler32_matched s2 adler2})
+  (len2: U32.t{U32.v len2 == Ghost.reveal m2}) =
+  adler32_combine64 s1 s2 adler1 adler2 (Cast.uint32_to_uint64 len2)
